### how to determine the distance between the two line in graph?

To determine the distance between two lines in a graph, we need to follow specific steps depending on whether the lines are in 2D or 3D space, and whether they are parallel, intersecting, or skew lines. Here's a detailed method for calculating the distance between two lines in both 2D and 3D graphs:

### For 2D Space:

**Given:**
1. Line 1: $` ax + by + c_1 = 0 `$
2. Line 2: $` ax + by + c_2 = 0 `$

**Solution By Steps**

**Step 1: Identify the Coefficients**

For the lines:
$` ax + by + c_1 = 0 `$
$` ax + by + c_2 = 0 `$

Identify the coefficients $`a`$, $`b`$, $`c_1`$, and $`c_2`$.

**Step 2: Use the Distance Formula**

The formula to find the distance $`d`$ between two parallel lines in 2D is:

$` d = \frac{|c_2 - c_1|}{\sqrt{a^2 + b^2}} `$

**Step 3: Calculate the Distance**

Substitute the values of $`a`$, $`b`$, $`c_1`$, and $`c_2`$ into the formula and solve for $`d`$.

**Final Answer**

$` d = \frac{|c_2 - c_1|}{\sqrt{a^2 + b^2}} `$

### How to determine the intersection point of two lines in 2D graph?

To determine the intersection point of two lines in a 2D graph, you need to find the point where the equations of the lines are satisfied simultaneously. Here's the step-by-step process to find the intersection point of two lines:

### Given:
1. Line 1: $`a_1x + b_1y + c_1 = 0`$
2. Line 2: $`a_2x + b_2y + c_2 = 0`$

### **Solution By Steps**

**Step 1: Set Up the System of Equations**

You have two linear equations:
$` a_1x + b_1y + c_1 = 0 `$
$` a_2x + b_2y + c_2 = 0 `$

**Step 2: Solve the System of Equations**

There are different methods to solve the system of linear equations: substitution, elimination, or using matrices. Here, we will use the elimination method.

**Step 3: Eliminate One Variable**

Multiply each equation by a suitable constant so that the coefficients of one of the variables become equal (but with opposite signs). Let's eliminate $`y`$:

Multiply Line 1 by $`b_2`$:
$` b_2a_1x + b_2b_1y + b_2c_1 = 0 `$

Multiply Line 2 by $`b_1`$:
$` b_1a_2x + b_1b_2y + b_1c_2 = 0 `$

**Step 4: Subtract the Equations**

Subtract the second equation from the first to eliminate $`y`$:
$` b_2a_1x - b_1a_2x + b_2c_1 - b_1c_2 = 0 `$

Simplify to solve for $`x`$:
$` x(b_2a_1 - b_1a_2) = b_1c_2 - b_2c_1 `$
$` x = \frac{b_1c_2 - b_2c_1}{b_2a_1 - b_1a_2} `$

**Step 5: Substitute $`x`$ Back to Find $`y`$**

Substitute the value of $`x`$ into one of the original equations to find $`y`$. Using Line 1:
$` a_1x + b_1y + c_1 = 0 `$
$` a_1\left(\frac{b_1c_2 - b_2c_1}{b_2a_1 - b_1a_2}\right) + b_1y + c_1 = 0 `$

Solve for $`y`$:
$` b_1y = -a_1\left(\frac{b_1c_2 - b_2c_1}{b_2a_1 - b_1a_2}\right) - c_1 `$
$` y = \frac{-a_1(b_1c_2 - b_2c_1) - c_1(b_2a_1 - b_1a_2)}{b_1(b_2a_1 - b_1a_2)} `$
$` y = \frac{(a_1b_2c_1 - a_1b_1c_2) - c_1b_2a_1 + c_1b_1a_2}{b_1(b_2a_1 - b_1a_2)} `$
$` y = \frac{a_1b_2c_1 - a_1b_1c_2 + c_1b_1a_2 - c_1b_2a_1}{b_1(b_2a_1 - b_1a_2)} `$
$` y = \frac{a_1b_2c_1 - a_1b_1c_2 + c_1(b_1a_2 - b_2a_1)}{b_1(b_2a_1 - b_1a_2)} `$

**Step 6: Intersection Point**

The intersection point $`P(x, y)`$ is:
$` P\left( \frac{b_1c_2 - b_2c_1}{b_2a_1 - b_1a_2}, \frac{a_1b_2c_1 - a_1b_1c_2 + c_1(b_1a_2 - b_2a_1)}{b_1(b_2a_1 - b_1a_2)} \right) `$

**Final Answer**

The intersection point of the two lines is:
$` \left( \frac{b_1c_2 - b_2c_1}{b_2a_1 - b_1a_2}, \frac{a_1b_2c_1 - a_1b_1c_2 + c_1(b_1a_2 - b_2a_1)}{b_1(b_2a_1 - b_1a_2)} \right) `$

### Example

**Given Lines:**
$` 2x + 3y - 6 = 0 `$
$` 4x - y - 1 = 0 `$

**Step-by-Step Calculation:**

1. Identify the coefficients: $`a_1 = 2`$, $`b_1 = 3`$, $`c_1 = -6`$, $`a_2 = 4`$, $`b_2 = -1`$, $`c_2 = -1`$.
2. Use the formula for $`x`$:

$` x = \frac{b_1c_2 - b_2c_1}{b_2a_1 - b_1a_2} = \frac{3(-1) - (-1)(-6)}{(-1)(2) - 3(4)} = \frac{-3 - 6}{-2 - 12} = \frac{-9}{-14} = \frac{9}{14} `$

3. Substitute $`x`$ back to find $`y`$:

$` 2x + 3y - 6 = 0 `$
$` 2\left(\frac{9}{14}\right) + 3y - 6 = 0 `$
$` \frac{18}{14} + 3y - 6 = 0 `$
$` \frac{9}{7} + 3y - 6 = 0 `$
$` 3y = 6 - \frac{9}{7} `$
$` 3y = \frac{42}{7} - \frac{9}{7} `$
$` 3y = \frac{33}{7} `$
$` y = \frac{33}{21} = \frac{11}{7} `$

**Intersection Point:**

$` \left( \frac{9}{14}, \frac{11}{7} \right) `$

**Key Concept**

- **Intersection of Two Lines**: The point where two lines meet, found by solving their equations simultaneously.

**Key Concept Explanation**

- **Solving Simultaneous Equations**: By setting up a system of linear equations, you can find the values of $`x`$ and $`y`$ that satisfy both equations, representing the intersection point of the lines.

**Related Knowledge or Questions**
[1] How to determine the slope of a line given its equation?
[2] How to find the equation of a line passing through two given points?
[3] How to determine if two lines are parallel or perpendicular?

You've done great exploring line intersections! Feel free to ask about any related topics or other questions you have!


### How to determine the perpendicular distance from a point to a line?
To determine the perpendicular distance from a point to a line in 2D space, you can use the formula derived from the line equation and the coordinates of the point. Here's a detailed explanation and step-by-step method:

### Given:
1. A line equation: $` ax + by + c = 0 `$
2. A point: $` (x_1, y_1) `$

### **Solution By Steps**

**Step 1: Identify the Coefficients and Point Coordinates**

For the line equation $` ax + by + c = 0 `$, identify the coefficients $` a `$, $` b `$, and $` c `$.

For the point $` (x_1, y_1) `$, identify the coordinates $` x_1 `$ and $` y_1 `$.

**Step 2: Use the Distance Formula**

The formula to find the perpendicular distance $` d `$ from the point $` (x_1, y_1) `$ to the line $` ax + by + c = 0 `$ is:

$` d = \frac{|ax_1 + by_1 + c|}{\sqrt{a^2 + b^2}} `$

**Step 3: Calculate the Distance**

Substitute the values of $` a `$, $` b `$, $` c `$, $` x_1 `$, and $` y_1 `$ into the formula and solve for $` d `$.

### Example

**Given Line:**
$` 3x + 4y - 5 = 0 `$

**Given Point:**
$` (2, 3) `$

**Step-by-Step Calculation:**

1. Identify the coefficients and coordinates:
   - $` a = 3 `$
   - $` b = 4 `$
   - $` c = -5 `$
   - $` x_1 = 2 `$
   - $` y_1 = 3 `$

2. Use the distance formula:

$` d = \frac{|3(2) + 4(3) - 5|}{\sqrt{3^2 + 4^2}} `$

3. Simplify the numerator:

$` d = \frac{|6 + 12 - 5|}{\sqrt{9 + 16}} `$
$` d = \frac{|13|}{\sqrt{25}} `$
$` d = \frac{13}{5} `$
$` d = 2.6 `$

### Final Answer

The perpendicular distance from the point $` (2, 3) `$ to the line $` 3x + 4y - 5 = 0 `$ is $` 2.6 `$.

**Key Concept**

- **Perpendicular Distance from a Point to a Line**: The shortest distance from a point to a line, measured along a line perpendicular to the given line.

**Key Concept Explanation**

- **Formula Derivation**: The formula $` d = \frac{|ax_1 + by_1 + c|}{\sqrt{a^2 + b^2}} `$ comes from the general equation of a line and the geometric concept of distance. It measures the absolute value of the line equation evaluated at the point, normalized by the length of the vector perpendicular to the line.

**Related Knowledge or Questions**
[1] How to find the equation of a line perpendicular to a given line passing through a specific point?
[2] How to determine the intersection point of two perpendicular lines?
[3] How to calculate the distance between two points in a 2D plane?

You've done great exploring the concept of perpendicular distance! If you want to learn more about related topics or have other questions, feel free to ask!


###  point‚Äìslope equation
The point-slope form of a linear equation is used to describe a line when you know a point on the line and the slope of the line. It's expressed as:

$` y - y_1 = m(x - x_1) `$

where:
- $` (x_1, y_1) `$ is a point on the line.
- $` m `$ is the slope of the line.

This form is particularly useful for writing the equation of a line when you have a specific point and the slope. If you know the slope and a point through which the line passes, you can easily plug these values into the formula.

### a  straight line passing through the points ùêµ ( 6 , ‚àí 4 ) and ùê∂ ( 9 , ‚àí 5 ) , what is the equation for this line ?
To find the equation of the line passing through the points $` B(6, -4) `$ and $` C(9, -5) `$, follow these steps:

1. **Find the slope (m):**

   The slope $` m `$ is given by:
   $`
   m = \frac{y_2 - y_1}{x_2 - x_1}
   `$
   Substituting the coordinates $` (x_1, y_1) = (6, -4) `$ and $` (x_2, y_2) = (9, -5) `$:
   $`
   m = \frac{-5 - (-4)}{9 - 6} = \frac{-5 + 4}{3} = \frac{-1}{3}
   `$

2. **Use the point-slope form of the equation:**

   Choose one of the points to use in the point-slope form. We'll use point $` B(6, -4) `$:
   $`
   y - y_1 = m(x - x_1)
   `$
   Substituting $` (x_1, y_1) = (6, -4) `$ and $` m = -\frac{1}{3} `$:
   $`
   y - (-4) = -\frac{1}{3}(x - 6)
   `$
   Simplify:
   $`
   y + 4 = -\frac{1}{3}(x - 6)
   `$
   $`
   y + 4 = -\frac{1}{3}x + 2
   `$
   $`
   y = -\frac{1}{3}x + 2 - 4
   `$
   $`
   y = -\frac{1}{3}x - 2
   `$

So, the equation of the line passing through the points $` B(6, -4) `$ and $` C(9, -5) `$ is:

$` y = -\frac{1}{3}x - 2 `$
